reflexivity & symmetry & transitivity

GroundZero/Meta/Notation.lean
@@ -1,19 +1,6 @@
 import Lean.Parser import Lean.Elab.Command
 open Lean.Parser Lean.Parser.Term Lean.Elab.Command
 
-section
-  variable {α : Type u} (ρ : α → α → Type v)
-
-  class Reflexive :=
-  (intro : ρ a a)
-
-  class Symmetric :=
-  (intro : ρ a b → ρ b a)
-
-  class Transitive :=
-  (intro : ρ a b → ρ b c → ρ a c)
-end
-
 namespace GroundZero.Meta.Notation
 
 syntax "Π" many1(simpleBinder <|> bracketedBinder) ", " term : term
@@ -24,12 +11,6 @@ macro xs:many1(funBinder) " ↦ " f:term : term => `(fun $xs* => $f)
 
 macro "begin " ts:sepBy1(tactic, ";", "; ", allowTrailingSep) i:"end" : term =>
   `(by { $[($ts:tactic)]* }%$i)
-
-section
-  macro "reflexivity"  : tactic => `(apply Reflexive.intro)
-  macro "symmetry"     : tactic => `(apply Symmetric.intro)
-  macro "transitivity" : tactic => `(apply Transitive.intro)
-end
 
 declare_syntax_cat superscriptNumeral
 syntax "⁰" : superscriptNumeral
