GroundZero/Meta/Tactic.lean
@@ -1,0 +1,54 @@
+import Lean.Elab.Command
+open Lean
+
+section
+  variable {α : Sort u} (ρ : α → α → Sort v)
+
+  class Reflexive :=
+  (intro (a : α) : ρ a a)
+
+  class Symmetric :=
+  (intro (a b : α) : ρ a b → ρ b a)
+
+  class Transitive :=
+  (intro (a b c : α) : ρ a b → ρ b c → ρ a c)
+end
+
+-- https://github.com/leanprover-community/mathlib4/blob/master/Mathlib/Lean/Expr/Basic.lean#L100-L109
+def Lean.Expr.constName (e : Expr) : Name :=
+e.constName?.getD Name.anonymous
+
+def Lean.Expr.getAppFnArgs (e : Expr) : Name × Array Expr :=
+withApp e λ e a => (e.constName, a)
+
+namespace GroundZero.Meta.Tactic
+
+-- https://github.com/leanprover-community/mathlib4/blob/master/Mathlib/Tactic/Ring.lean#L411-L419
+def applyOnBinRel (n : Lean.Name) : Elab.Tactic.TacticM Unit := do
+  let mvars ← Elab.Tactic.liftMetaMAtMain (λ mvar => do
+    let ε ← Meta.instantiateMVars (← Meta.getMVarDecl mvar).type
+    ε.withApp λ e es => do
+      if ¬(es.size > 1) then throwError "expected binary relation"
+
+      let e₂ := es.back; let es := es.pop;
+      let e₁ := es.back; let es := es.pop;
+
+      let ty  ← Meta.inferType e₁
+      let ty' ← Meta.inferType e₂
+
+      if ¬(← Meta.isDefEq ty ty') then throwError "{ty} ≠ {ty'}"
+
+      let u ← Meta.getLevel ty
+      let v ← Meta.getLevel ε
+
+      mkApp2 (mkConst n [u, v]) ty (mkAppN e es)
+      |> Meta.apply mvar)
+  Lean.Elab.Tactic.replaceMainGoal mvars
+
+section
+  elab "reflexivity"  : tactic => applyOnBinRel `Reflexive.intro
+  elab "symmetry"     : tactic => applyOnBinRel `Symmetric.intro
+  elab "transitivity" : tactic => applyOnBinRel `Transitive.intro
+end
+
+end GroundZero.Meta.Tactic
